Prove semantic typing of dividing by positive numbers

theories/Dot/examples/examples.v
@@ -1,7 +1,27 @@
 From iris.proofmode Require Import tactics.
+From D.pure_program_logic Require Import lifting adequacy.
 From D.Dot Require Import unary_lr
-  lr_lemmas lr_lemmasNoBinding lr_lemmasDefs.
-From D.Dot Require Import exampleInfra typingExInfra.
+  lr_lemmas lr_lemmasNoBinding lr_lemmasDefs lr_lemmasPrim.
+From D.Dot Require Import skeleton fundamental.
+From D.Dot Require Import scalaLib hoas exampleInfra typingExInfra.
+
+Import hoasNotation.
+
+Example loopDefTyp Γ : Γ v⊢ₜ[ ∅ ] hclose (htv hloopDefV) : hclose hloopDefT.
+Proof.
+  apply (Subs_typed_nocoerce (hclose hloopDefTConcr)); mltcrush. cbv.
+
+  eapply App_typed; last var.
+  tcrush; varsub; lookup.
+Qed.
+
+Example loopFunTyp Γ : Γ v⊢ₜ[∅] hclose hloopFunTm : hclose ⊤ →: ⊥.
+Proof. have ? := loopDefTyp Γ; tcrush. Qed.
+
+Example loopTyp Γ : Γ v⊢ₜ[∅] hclose hloopTm : ⊥.
+Proof.
+  have ? := loopFunTyp Γ; apply (App_typed (T1 := ⊤)), (Subs_typed_nocoerce 𝐍); tcrush.
+Qed.
 
 (** XXX Not currently using olty. *)
 Module example.
@@ -18,7 +38,54 @@ Section ex.
 
   Definition pos v := ∃ n, v = vnat n ∧ n > 0.
   Definition ipos: envD Σ := λ ρ v, (⌜ pos v ⌝) %I.
-  Instance posP ρ v: Persistent (ipos ρ v) := _.
+  Import ectxi_language ectx_language.
+
+(* Arguments dlang_ectx_lang : simpl never.
+Arguments dlang_ectxi_lang : simpl never. *)
+
+  Ltac wp_bin_base := iApply wp_bin; first eapply bin_op_syntype_sound; by [|constructor].
+  Ltac wp_bin := iApply wp_wand; [wp_bin_base | iIntros].
+  Tactic Notation "wp_bind" uconstr(p) := iApply (wp_bind (fill [p])).
+
+  Lemma wp_ge m n (Hge : m > n) : WP m > n {{ w, w ≡ true }}%I.
+  Proof. wp_bin. ev; simplify_eq/=. by case_decide. Qed.
+  Lemma wp_nge m n (Hnge : ¬ m > n) : WP m > n {{ w, w ≡ false }}%I.
+  Proof. wp_bin. ev; simplify_eq/=. by case_decide. Qed.
+
+  Lemma pos_wp ρ v : ipos ρ v ⊢ WP v > 0 {{ w, w ≡ vbool true }}.
+  Proof. iDestruct 1 as %(n & -> & ?). by iApply wp_ge. Qed.
+
+  Import swap_later_impl.
+  Context `{SwapPropI Σ}.
+  Lemma loopSemT: (WP hclose hloopTm {{ _, False }})%I.
+  Proof.
+    iDestruct (fundamental_typed _ _ _ _ (loopTyp []) with "[]") as "H".
+    iApply wellMappedφ_empty.
+    iSpecialize ("H" $! ids with "[//]").
+    by rewrite hsubst_id /=.
+  Qed.
+
+  Definition hmkPosBodyV n := htif (n > 0) n hloopTm.
+  Definition hmkPosV := λ: n, hmkPosBodyV n.
+  Lemma wp_if_ge (n : nat) :
+    WP hclose (hmkPosBodyV n) {{ w, ⌜ w = n ∧ n > 0 ⌝}}%I.
+  Proof.
+    wp_bind (IfCtx _ _).
+    wp_bin; ev; simplify_eq/=.
+    case_decide; rewrite -wp_pure_step_later //; iNext.
+    by rewrite -wp_value'.
+    iApply wp_wand; [iApply loopSemT | naive_solver].
+  Qed.
+
+  Lemma wp_if_ge' (n : nat) :
+    WP tif (n > 0) (1 `div` n) (hclose hloopTm) {{ w, ⟦ 𝐍 ⟧ ids w ∧ ⌜ n > 0 ⌝}}%I.
+  Proof.
+    wp_bind (IfCtx _ _).
+    wp_bin; ev; simplify_eq/=.
+    case_decide; rewrite -wp_pure_step_later //; iNext.
+    - wp_bin. naive_solver.
+    - iApply wp_wand; [iApply loopSemT | naive_solver].
+  Qed.
 
   Context (s: stamp).
 
@@ -42,30 +109,6 @@ Section ex.
     by rewrite lookup_insert.
   Qed.
 
-  (** Under Iris assumption [Hs], [v.A] points to [ipos].
-      We assume [Hs] throughout the rest of the section. *)
-  Import DBNotation.
-
-  Definition v := ν {@
-    type "A" = ([]; s);
-	  val "n" = pv (vnat 2)
-  }.
-
-  Lemma sHasA : Hs -∗ def_interp_tmem ⟦ ⊥ ⟧ ⟦ 𝐍 ⟧ ids (dtysem [] s).
-  Proof.
-    iIntros; cbn; repeat (repeat iExists _; repeat iSplit; try done).
-    by iApply dm_to_type_intro.
-    iModIntro; repeat iSplit; iIntros (w). by iIntros ">[]".
-    iMod 1 as %(n & -> & ?). iPureIntro.
-    rewrite /pure_interp_prim /prim_evals_to /=. eauto.
-  Qed.
-
-  (** Yes, v has a valid type member. *)
-  Lemma vHasA0: Hs -∗ ∀ ρ, ⟦ type "A" >: ⊥ <: TNat ⟧ ρ v.[ρ].
-  Proof.
-    iIntros "#Hs" (ρ); iExists _; iSplit; by [eauto | iApply sHasA].
-  Qed.
-
   (* Generic useful lemmas — not needed for fundamental theorem,
      but very useful for examples. *)
   Lemma ietp_value T v: (∀ ρ, ⟦ T ⟧ ρ v.[ρ]) -∗ [] ⊨ tv v : T.
@@ -81,6 +124,63 @@ Section ex.
     by rewrite wp_value_inv'.
   Qed.
 
+
+  Import hoasNotation.
+
+  Definition posModT := μ: self, {@
+    type "Pos" >: ⊥ <: 𝐍;
+    val "mkPos" : 𝐍 →: self @; "Pos";
+    val "div" : 𝐍 →: self @; "Pos" →: 𝐍
+  }.
+
+  Definition hdivV := λ: m n, (htskip m) `div` n.
+
+  (** Under Iris assumption [Hs], [v.A] points to [ipos].
+      We assume [Hs] throughout the rest of the section. *)
+  Import DBNotation.
+
+  Definition posModV := ν {@
+    type "Pos" = ([]; s);
+    val "mkPos" = pv (hclose hmkPosV);
+    val "div" = pv (hclose hdivV)
+  }.
+
+  Definition v := ν {@
+    type "A" = ([]; s);
+	  val "n" = pv (vnat 2)
+  }.
+
+  Lemma sToIpos : Hs -∗ dtysem [] s ↗ ipos (∞ []).
+  Proof. by iApply dm_to_type_intro. Qed.
+
+  Lemma sHasA : Hs -∗ def_interp_tmem ⟦ ⊥ ⟧ ⟦ 𝐍 ⟧ ids (dtysem [] s).
+  Proof.
+    iIntros; cbn; repeat (repeat iExists _; repeat iSplit; try done).
+    by iApply sToIpos.
+    iModIntro; repeat iSplit; iIntros (w). by iIntros ">[]".
+    iMod 1 as %(n & -> & ?). iPureIntro.
+    rewrite /pure_interp_prim /prim_evals_to /=. eauto.
+  Qed.
+
+  Lemma wp_mkPos :
+    interp_forall ⟦ 𝐍 ⟧ (λ ρ v, ⌜ ∃ n : nat, v = n ∧ n > 0 ⌝)%I ids (hclose hmkPosV).
+  Proof.
+    repeat (iExists _; iSplit => //).
+    iIntros (w) "!>"; iMod 1 as %[n Hw]; iIntros "!> !>".
+    simplify_eq/=.
+    iApply wp_wand; [iApply wp_if_ge | iIntros "!% /="].
+    naive_solver.
+  Qed.
+
+  (** Yes, v has a valid type member. *)
+  Lemma vHasA0: Hs -∗ ∀ ρ, ⟦ type "A" >: ⊥ <: TNat ⟧ ρ v.[ρ].
+  Proof.
+    iIntros "#Hs" (ρ); iExists _; iSplit; by [eauto | iApply sHasA].
+  Qed.
+
+  Lemma posModVHasA0: Hs -∗ ∀ ρ, ⟦ type "Pos" >: ⊥ <: TNat ⟧ ρ posModV.[ρ].
+  Proof. iIntros "#Hs" (ρ); iExists _; iSplit; by [eauto | iApply sHasA]. Qed.
+
   Lemma vHasA0typ: Hs -∗ [] ⊨ tv v : type "A" >: ⊥ <: 𝐍.
   Proof. rewrite -ietp_value. iApply vHasA0. Qed.
 
@@ -88,6 +188,59 @@ Section ex.
     type "A" >: ⊥ <: 𝐍;
     val "n" : p0 @; "A"
   }.
+
+  Lemma wp_div_spec (m : nat) w : ipos ids w -∗ WP m `div` w {{ ⟦ 𝐍 ⟧ ids }}.
+  Proof. iDestruct 1 as %(n&?&?); simplify_eq. wp_bin. by iIntros "!%"; naive_solver. Qed.
+
+  Lemma V_TVMem_I T (v w : vl) l
+    (Hclv : nclosed_vl v 0)
+    (* XXX should be (Hlook : w @ l ↘ (dpt (pv v))) *)
+    (Hlook : objLookup v l (dpt (pv w))):
+    [] ⊨ tv w : T -∗
+    [] ⊨ v : TVMem l T.
+  Proof.
+    Import synLemmas.
+    have Hclw: nclosed_vl w 0.
+    by have := nclosed_lookup' Hlook Hclv; eauto with fv.
+    iIntros "#H"; iApply ietp_value; iIntros (ρ) "/=".
+    iSpecialize ("H" $! ρ with "[//]"). rewrite wp_value_inv.
+    rewrite !closed_subst_vl_id //.
+    do 2 (iExists _; iSplit; [done|]).
+    by rewrite path_wp_pv.
+  Qed.
+
+  Ltac valMember ρ :=
+    iApply V_TVMem_I; [solve_fv_congruence|naive_solver|
+      rewrite -ietp_value; iIntros (ρ)].
+
+  Lemma posModVHasA: Hs -∗ [] ⊨ posModV : hclose posModT.
+  Proof.
+    rewrite /posModT -(TMu_I [] _ posModV).
+    iIntros "#Hs". cbn -[ietp].
+    iApply TAnd_I; first by rewrite -ietp_value -posModVHasA0.
+    iApply TAnd_I; last iApply TAnd_I; last by
+      iIntros "!> ** /="; rewrite -wp_value'.
+    - valMember ρ; iExists _; iSplit; [done|].
+      iIntros (w) "!>"; iMod 1 as %[n Hw]; iIntros "!> !>".
+      simplify_eq/=.
+      iApply wp_wand; [iApply wp_if_ge | iIntros "/=" (v [-> ?])].
+      rewrite path_wp_pv.
+      repeat (iExists _; try iSplit => //=).
+      iSplit => //. by iApply dm_to_type_intro.
+      iIntros "!%"; rewrite /pos.
+      naive_solver.
+    - valMember ρ; iExists _; iSplit; [done|].
+      iIntros (v) "!>"; iMod 1 as %[m Hw]; iIntros "!> !>".
+      rewrite -wp_value'; simplify_eq/=; iExists _; iSplit; [done|].
+      iIntros (w) "!> #Harg!>!>"; rewrite path_wp_pv /=.
+      iDestruct "Harg" as (Φ d [ds Hlook]) "[Hs1 #Harg]";
+        have {d ds Hlook}->: d = dtysem [] s by naive_solver.
+      iPoseProof (sToIpos with "Hs") as "Hs2/=".
+      iPoseProof (dm_to_type_agree _ _ _ w with "Hs1 Hs2") as "{Hs Hs1 Hs2} Heq".
+      wp_bind (BinLCtx _ _); rewrite -wp_pure_step_later // -wp_value/=/lang.of_val.
+      iNext. iRewrite "Heq" in "Harg"; iClear "Heq".
+      by iApply wp_div_spec.
+  Qed.
 
   (* This works. Crucially, we use TMu_I to introduce the object type.
      This way, we can inline the object in the type selection.
@@ -118,6 +271,12 @@ Section ex.
 
   Lemma vHasA1TypAd : allGs ∅ ==∗ [] ⊨ tv v : vTyp1.
   Proof. rewrite -ietp_value allocHs //; iIntros. by iApply vHasA1. Qed.
+
+  (* Lemma vHasA1': Hs -∗ ∀ ρ, ⟦ vTyp1 ⟧ ρ v.[ρ].
+  Proof.
+    rewrite -ietp_value_inv. iIntros "#Hs".
+    (* Fails, because we need a *syntactic* type. *)
+    iApply (T_Sub [] v _ vTyp1 0). *)
 
   (*
     A different approach would be to type the object using T_New_I
@@ -156,6 +315,38 @@ Section ex.
       (* Last case is stuck, since we don't know what [ρ 0] is and what
       "A" points to. *)
   Abort.
+
+  Lemma wp_prim_step {e : tm} (Hne : to_val e = None) φ :
+    WP e {{ φ }} ⊢ ∃ e2, ⌜ prim_step e tt [] e2 tt [] ⌝ ∧ ▷ WP e2 {{ φ }}.
+  Proof.
+    rewrite wp_unfold/wp_pre/= {}Hne; iIntros "Hwp".
+    iDestruct ("Hwp" $! () [] [] 0 with "[//]") as (Hred) "Hwp".
+    destruct Hred as (? & e2 & [] & ? & Hr%prim_step_view).
+    iDestruct ("Hwp" $! e2 with "[%//]") as "(_ & Heq & _)".
+    by iExists _; iFrame.
+  Qed.
+
+  Lemma wp_head_step {e : tm} (Hsub : sub_redexes_are_values e) (Hne : to_val e = None) φ :
+    WP e {{ φ }} ⊢ ∃ e2 : tm, ⌜ head_step e tt [] e2 tt [] ⌝ ∧ ▷ WP e2 {{ φ }}.
+  Proof.
+    iIntros "H"; iDestruct (wp_prim_step Hne with "H") as (e2 Hred) "Hwp".
+    suff ?: head_step e () [] e2 () [] by iExists _; iFrame.
+    destruct Hred as [K]; subst; suff: K = [] by naive_solver.
+    by eapply Hsub, val_head_stuck.
+  Qed.
+
+  Lemma wp_pos ρ (v : vl) : WP v > 0 {{ w, w ≡ vbool true }} ⊢ ▷ ipos ρ v.
+  Proof.
+    have Hsub: sub_redexes_are_values (v > 0). {
+      apply ectxi_language_sub_redexes_are_values.
+      by case => /= *; simplify_eq/=; eauto.
+    }
+    rewrite /ipos/pos (wp_head_step Hsub) //; iDestruct 1 as (e2 Hhr) "Heq"; iNext.
+    have {Hhr}[w [-> Hev]]: ∃ w : vl, e2 = w ∧ bin_op_eval blt 0 v = Some w by inverse Hhr; eauto.
+    iDestruct (wp_value_inv' with "Heq") as %->%leibniz_equiv; iIntros "!%".
+    (* rewrite wp_value_inv'; iDestruct "Heq" as %->%leibniz_equiv; iIntros "!%". *)
+    simpl in Hev; repeat case_match; repeat case_decide; naive_solver.
+  Qed.
 
 End ex.
 
